common/LanguageInterface.v
@@ -1,0 +1,84 @@
+Require Import AST.
+Require Import Globalenvs.
+
+(** * Semantic interface of languages *)
+
+Structure language_interface :=
+  mk_language_interface {
+    query: Type;
+    reply: Type;
+  }.
+
+(** ** Null interface *)
+
+(** The null language interface defined below is used as the outgoing
+  interface for closed semantics. *)
+
+Definition li_null :=
+  {|
+    query := Empty_set;
+    reply := Empty_set;
+  |}.
+
+(** * Calling conventions *)
+
+(** ** Definition *)
+
+Record callconv li1 li2 :=
+  mk_callconv {
+    ccworld : Type;
+    match_senv: ccworld -> Senv.t -> Senv.t -> Prop;
+    match_query: ccworld -> query li1 -> query li2 -> Prop;
+    match_reply: ccworld -> reply li1 -> reply li2 -> Prop;
+    match_senv_public_preserved:
+      forall w se1 se2,
+        match_senv w se1 se2 ->
+        forall id, Senv.public_symbol se2 id = Senv.public_symbol se1 id;
+  }.
+
+Arguments ccworld {_ _}.
+Arguments match_senv {_ _} _ _ _.
+Arguments match_query {_ _} _ _ _.
+Arguments match_reply {_ _} _ _ _.
+
+Delimit Scope cc_scope with cc.
+Bind Scope cc_scope with callconv.
+Local Obligation Tactic := cbn; eauto.
+
+(** ** Identity *)
+
+Program Definition cc_id {li}: callconv li li :=
+  {|
+    ccworld := unit;
+    match_senv w := eq;
+    match_query w := eq;
+    match_reply w := eq;
+  |}.
+Next Obligation.
+  congruence.
+Qed.
+
+(** ** Composition *)
+
+Program Definition cc_compose {li1 li2 li3} (cc12: callconv li1 li2) (cc23: callconv li2 li3) :=
+  {|
+    ccworld := ccworld cc12 * ccworld cc23;
+    match_senv w se1 se3 :=
+      exists se2,
+        match_senv cc12 (fst w) se1 se2 /\
+        match_senv cc23 (snd w) se2 se3;
+    match_query w q1 q3 :=
+      exists q2,
+        match_query cc12 (fst w) q1 q2 /\
+        match_query cc23 (snd w) q2 q3;
+    match_reply w r1 r3 :=
+      exists r2,
+        match_reply cc12 (fst w) r1 r2 /\
+        match_reply cc23 (snd w) r2 r3;
+  |}.
+Next Obligation.
+  intros li1 li2 li3 cc12 cc23 w se1 se3 (se2 & H12 & H23) id.
+  etransitivity; eauto using match_senv_public_preserved.
+Qed.
+
+Infix "@" := cc_compose (at level 30, right associativity) : cc_scope.
